WIP

pcuic/theories/PCUICConversionDef.v
@@ -3,7 +3,6 @@ From MetaCoq.Template Require Import config utils monad_utils EnvironmentTyping.
 From MetaCoq.PCUIC Require Import PCUICAst PCUICAstUtils PCUICLiftSubst
      PCUICUnivSubst PCUICEquality PCUICUtils PCUICPosition.
 
-Require Import ssreflect.
 Set Asymmetric Patterns.
 Require Import Equations.Type.Relation.
 From Equations Require Import Equations.
@@ -90,7 +89,7 @@ Proof.
 Qed.
 
 Lemma fix_context_length mfix : #|fix_context mfix| = #|mfix|.
-Proof. unfold fix_context. now rewrite List.rev_length mapi_length. Qed.
+Proof. unfold fix_context. now rewrite List.rev_length, mapi_length. Qed.
 
 Definition tDummy := tVar ""%string.
 
@@ -343,14 +342,6 @@ Proof.
       constructor; try split; auto; intuition.
 Defined.
 
-(** *** Reduction
-
-  The reflexive-transitive closure of 1-step reduction. *)
-
-Inductive red Σ Γ M : term -> Type :=
-| refl_red : red Σ Γ M M
-| trans_red : forall (P : term) N, red Σ Γ M P -> red1 Σ Γ P N -> red Σ Γ M N.
-
 
 
 (** ** η Expansion *)
@@ -519,8 +510,13 @@ Proof.
 Defined.
 
 
+Definition red Σ Γ := clos_refl_trans (red1 Σ Γ).
+
 (* [eta u v] states v is a reduction of u *)
 Definition eta := clos_refl_trans eta1.
+
+Definition beta_eta1 Σ Γ := union (red1 Σ Γ) eta1.
+Definition beta_eta Σ Γ := clos_refl_trans (beta_eta1 Σ Γ).
 
 
 
@@ -529,32 +525,60 @@ Definition eta := clos_refl_trans eta1.
 (** Two terms are in cumulativity/conversion relation if they β-reduce/η-expand
     to two equal terms up to universes and in the cumul/conv relation *)   
 
-Reserved Notation " Σ ;;; Γ |- t <= u " (at level 50, Γ, t, u at next level).
-Reserved Notation " Σ ;;; Γ |- t = u " (at level 50, Γ, t, u at next level).
+Definition cumul `{checker_flags} (Σ : global_env_ext) (Γ : context) (t u : term)
+  := ∑ t' t'' u' u'', upto_domain t t' ×
+                      beta_eta Σ Γ t' t'' ×
+                      leq_term Σ t'' u'' ×
+                      beta_eta Σ Γ u' u'' ×
+                      upto_domain u u'.
 
-Inductive cumul `{checker_flags} (Σ : global_env_ext) (Γ : context) : term -> term -> Type :=
-| cumul_refl t u v : leq_term (global_ext_constraints Σ) t u -> upto_domain u v -> Σ ;;; Γ |- t <= v
-| cumul_red_l t u v : red1 Σ.1 Γ t v -> Σ ;;; Γ |- v <= u -> Σ ;;; Γ |- t <= u
-| cumul_red_r t u v : Σ ;;; Γ |- t <= v -> red1 Σ.1 Γ u v -> Σ ;;; Γ |- t <= u
-| cumul_eta_l t u v : eta1 t v -> Σ ;;; Γ |- v <= u -> Σ ;;; Γ |- t <= u
-| cumul_eta_r t u v : Σ ;;; Γ |- t <= v -> eta1 u v -> Σ ;;; Γ |- t <= u
-where " Σ ;;; Γ |- t <= u " := (cumul Σ Γ t u) : type_scope.
+Definition conv `{checker_flags} (Σ : global_env_ext) (Γ : context) (t u : term)
+  := ∑ t' t'' u' u'', upto_domain t t' ×
+                      beta_eta Σ Γ t' t'' ×
+                      eq_term Σ t'' u'' ×
+                      beta_eta Σ Γ u' u'' ×
+                      upto_domain u u'.
 
-
-Inductive conv `{checker_flags} (Σ : global_env_ext) (Γ : context) : term -> term -> Type :=
-| conv_refl t u v : eq_term (global_ext_constraints Σ) t u -> upto_domain u v -> Σ ;;; Γ |- t = v
-| conv_red_l t u v : red1 Σ Γ t v -> Σ ;;; Γ |- v = u -> Σ ;;; Γ |- t = u
-| conv_red_r t u v : Σ ;;; Γ |- t = v -> red1 (fst Σ) Γ u v -> Σ ;;; Γ |- t = u
-| conv_eta_l t u v : eta1 t v -> Σ ;;; Γ |- v = u -> Σ ;;; Γ |- t = u
-| conv_eta_r t u v : Σ ;;; Γ |- t = v -> eta1 u v -> Σ ;;; Γ |- t = u
-where " Σ ;;; Γ |- t = u " := (@conv _ Σ Γ t u) : type_scope.
-
-Hint Resolve cumul_refl conv_refl : pcuic.
+Notation " Σ ;;; Γ |- t <= u " := (cumul Σ Γ t u) (at level 50, Γ, t, u at next level).
+Notation " Σ ;;; Γ |- t = u " := (conv Σ Γ t u) (at level 50, Γ, t, u at next level).
 
 
-(** ** Basic Properties of eta *)
 
-(* todo *)
+(** ** Basic Properties of beta *)
+
+(* todo move *)
+Instance clos_refl_trans_refl {A} (R : relation A) : Reflexive (clos_refl_trans R).
+Proof. constructor 2. Defined.
+
+Instance clos_refl_trans_trans {A} (R : relation A)
+  : Transitive (clos_refl_trans R).
+Proof. econstructor 3; eassumption. Defined.
+
+
+Lemma refl_red Σ Γ M : red Σ Γ M M.
+Proof. constructor 2. Qed.
+
+Lemma trans_red Σ Γ M N P : red Σ Γ M P -> red1 Σ Γ P N -> red Σ Γ M N.
+Proof.
+  intros. econstructor 3; tea.
+  now constructor.
+Qed.
+
+Lemma red1_red (Σ : global_env) Γ t u : red1 Σ Γ t u -> red Σ Γ t u.
+Proof. now constructor. Qed.
+Hint Resolve red1_red refl_red : core pcuic.
+
+
+Lemma red_step Σ Γ t u v : red1 Σ Γ t u -> red Σ Γ u v -> red Σ Γ t v.
+Proof.
+  intros; etransitivity; tea.
+  now constructor.
+Qed.
+
+Lemma red_trans Σ Γ t u v : red Σ Γ t u -> red Σ Γ u v -> red Σ Γ t v.
+Proof.
+  econstructor 3; tea.
+Defined.
 
 
 (** ** Basic Properties of eta *)
@@ -575,6 +599,12 @@ Instance eta_trans' : Transitive eta := eta_trans.
 Hint Constructors eta1 : eta.
 Hint Resolve eta1_eta eta_refl eta_trans : eta.
 
+Ltac eta := match goal with
+            | |- _ × _ => split
+            | _ => idtac 
+            end; auto with eta.
+
+
 (** *** Congruences for eta *)
 
 Lemma eta_Evar n l l' :
@@ -590,7 +620,7 @@ Proof.
     induction r; [econstructor 1|econstructor 2|econstructor 3];
       eauto with eta.
     constructor. apply OnOne2_app. now constructor.
-  - now rewrite (app_cons l0 l) (app_cons l0 l').
+  - now rewrite (app_cons l0 l), (app_cons l0 l').
 Defined.
 
 Lemma eta_Prod na M M' N N' :
@@ -651,7 +681,7 @@ Proof.
   transitivity (tCase indn p' c' (brs0 ++ (n0, t0) :: l)); eauto with eta.
   - induction r; [econstructor 1| | ]; eauto with eta.
     constructor. apply OnOne2_app. now constructor.
-  - now rewrite (app_cons brs0 l) (app_cons brs0 l').
+  - now rewrite (app_cons brs0 l), (app_cons brs0 l').
 Defined.
 
 Lemma eta_Case0 indn p c brs p' c' :
@@ -691,7 +721,7 @@ Proof.
                                   dbody := dbody0; rarg := rarg0 |} :: l) idx). {
     induction r0; [econstructor 1| | ]; eauto with eta.
     eapply fix_eta_body. apply OnOne2_app. now constructor. }
-  now rewrite (app_cons mfix0 l) (app_cons mfix0 l').
+  now rewrite (app_cons mfix0 l), (app_cons mfix0 l').
 Defined.
 
 Lemma eta_CoFix mfix mfix' idx :
@@ -715,7 +745,7 @@ Proof.
                                   dbody := dbody0; rarg := rarg0 |} :: l) idx). {
     induction r0; [econstructor 1| | ]; eauto with eta.
     eapply cofix_eta_body. apply OnOne2_app. now constructor. }
-  now rewrite (app_cons mfix0 l) (app_cons mfix0 l').
+  now rewrite (app_cons mfix0 l), (app_cons mfix0 l').
 Defined.
 
 Lemma eta_mkApps M M' l l' :
@@ -732,73 +762,482 @@ Hint Extern 0 (All2 _ _ _) => OnOne2_All2; intuition auto with eta : eta.
 Hint Resolve All2_refl : eta.
 
  
+(** ** Basic Properties of beta_eta *)
+
+Create HintDb beta_eta.
+
+Tactic Notation "beta_eta" integer(n) :=
+  repeat match goal with
+         | |- _ × _ => split
+         end;
+  match goal with
+  | |- upto_domain _ _ => eauto n with utd
+  | _ => idtac
+  end;
+  eauto n with beta_eta.
+
+Tactic Notation "beta_eta" := beta_eta 5.
+Hint Constructors eta1 : beta_eta.
+Hint Constructors red1 : beta_eta.
+
+Definition beta_eta_refl Σ Γ x : beta_eta Σ Γ x x := clos_refl_trans_refl _ _.
+Hint Resolve beta_eta_refl : beta_eta.
+
+Definition beta_eta_trans Σ Γ x y z :
+  beta_eta Σ Γ x y -> beta_eta Σ Γ y z -> beta_eta Σ Γ x z
+  := clos_refl_trans_trans _ x y z.
+Hint Resolve beta_eta_trans : beta_eta.
+
+Lemma red_beta_eta Σ Γ M N :
+  red Σ Γ M N -> beta_eta Σ Γ M N.
+Proof.
+  induction 1; try reflexivity.
+  - constructor. now left.
+  - etransitivity; tea.
+Defined.
+Hint Resolve red_beta_eta : beta_eta.
+
+Lemma eta_beta_eta Σ Γ M N :
+  eta M N -> beta_eta Σ Γ M N.
+Proof.
+  induction 1; try reflexivity.
+  - constructor. now right.
+  - etransitivity; tea.
+Defined.
+Hint Resolve eta_beta_eta : beta_eta.
+
+Hint Resolve eta1_eta : beta_eta.
+Hint Resolve red1_red : beta_eta.
+
+Lemma red1_beta_eta Σ Γ M N :
+  red1 Σ Γ M N -> beta_eta Σ Γ M N.
+Proof. beta_eta. Defined.
+
+Lemma eta1_beta_eta Σ Γ M N :
+  eta1 M N -> beta_eta Σ Γ M N.
+Proof. beta_eta. Defined.
+
+Lemma beta_eta_Evar Σ Γ n l l' :
+  All2 (beta_eta Σ Γ) l l' ->
+  beta_eta Σ Γ (tEvar n l) (tEvar n l').
+Proof.
+  intro X.
+  enough (forall l0, beta_eta Σ Γ (tEvar n (l0 ++ l)) (tEvar n (l0 ++ l'))) as XX;
+    [apply (XX [])|].
+  induction X; auto with beta_eta.
+  intro l0; transitivity (tEvar n (l0 ++ y :: l)); beta_eta.
+  - clear -r.
+    induction r; [econstructor 1|econstructor 2|econstructor 3]; beta_eta.
+    destruct r; [left|right]; constructor; apply OnOne2_app; now constructor.
+  - now rewrite (app_cons l0 l), (app_cons l0 l').
+Defined.
+Hint Resolve beta_eta_Evar : beta_eta.
+
+Lemma beta_eta_Prod Σ Γ na M M' N N' :
+  beta_eta Σ Γ M M' ->
+  beta_eta Σ (Γ ,, vass na M') N N' ->
+  beta_eta Σ Γ (tProd na M N) (tProd na M' N').
+Proof.
+  intros X Y; transitivity (tProd na M' N).
+  - clear Y. induction X; beta_eta.
+    destruct r; beta_eta.
+  - clear X. induction Y; beta_eta.
+    destruct r; beta_eta.
+Defined.
+Hint Resolve beta_eta_Prod : beta_eta.
+
+Lemma beta_eta_Lambda Σ Γ na M M' N N' :
+  beta_eta Σ Γ M M' ->
+  beta_eta Σ (Γ ,, vass na M') N N' ->
+  beta_eta Σ Γ (tLambda na M N) (tLambda na M' N').
+Proof.
+  intros X Y; transitivity (tLambda na M' N).
+  - clear Y. induction X; beta_eta.
+    destruct r; beta_eta.
+  - clear X. induction Y; beta_eta.
+    destruct r; beta_eta.
+Defined.
+Hint Resolve beta_eta_Lambda : beta_eta.
+
+Lemma beta_eta_LetIn Σ Γ na d0 d1 t0 t1 b0 b1 :
+  beta_eta Σ Γ d0 d1 -> beta_eta Σ Γ t0 t1 -> beta_eta Σ (Γ ,, vdef na d1 t1) b0 b1 ->
+  beta_eta Σ Γ (tLetIn na d0 t0 b0) (tLetIn na d1 t1 b1).
+Proof.
+  intros X Y Z;
+    transitivity (tLetIn na d1 t0 b0); [|transitivity (tLetIn na d1 t1 b0)].
+  - clear Y Z. induction X; beta_eta.
+    destruct r; beta_eta.
+  - clear X Z. induction Y; beta_eta.
+    destruct r; beta_eta.
+  - clear X Y. induction Z; beta_eta.
+    destruct r; beta_eta.
+Defined.
+Hint Resolve beta_eta_LetIn : beta_eta.
+
+Lemma beta_eta_App Σ Γ M M' N N' :
+  beta_eta Σ Γ M M' ->
+  beta_eta Σ Γ N N' ->
+  beta_eta Σ Γ (tApp M N) (tApp M' N').
+Proof.
+  intros X Y; transitivity (tApp M' N).
+  - clear Y. induction X; beta_eta.
+    destruct r; beta_eta.
+  - clear X. induction Y; beta_eta.
+    destruct r; beta_eta.
+Defined.
+Hint Resolve beta_eta_App : beta_eta.
+
+Lemma beta_eta_Case Σ Γ indn p c brs p' c' brs' :
+  beta_eta Σ Γ p p' ->
+  beta_eta Σ Γ c c' ->
+  All2 (on_Trel_eq (beta_eta Σ Γ) snd fst) brs brs' ->
+  beta_eta Σ Γ (tCase indn p c brs) (tCase indn p' c' brs').
+Proof.
+  intros X Y Z.
+  transitivity (tCase indn p' c brs). {
+    induction X; beta_eta. destruct r; beta_eta. }
+  transitivity (tCase indn p' c' brs). {
+    induction Y; beta_eta. destruct r; beta_eta. }
+  clear -Z.
+  enough (forall brs0, beta_eta Σ Γ (tCase indn p' c'  (brs0 ++ brs))
+                               (tCase indn p' c'  (brs0 ++ brs'))) as XX;
+    [apply (XX [])|].
+  induction Z; beta_eta.
+  destruct x as [n ?], y as [n0 ?], r as [r ?]; cbn in *; subst.
+  intro brs0.
+  transitivity (tCase indn p' c' (brs0 ++ (n0, t0) :: l)); beta_eta.
+  - induction r; [econstructor 1| | ]; beta_eta.
+    destruct r; [left|right];
+    constructor; apply OnOne2_app; now constructor.
+  - now rewrite (app_cons brs0 l), (app_cons brs0 l').
+Defined.
+Hint Resolve beta_eta_Case : beta_eta.
+
+Lemma beta_eta_Case0 Σ Γ indn p c brs p' c' :
+  beta_eta Σ Γ p p' ->
+  beta_eta Σ Γ c c' ->
+  beta_eta Σ Γ (tCase indn p c brs) (tCase indn p' c' brs).
+Proof.
+  intros; apply beta_eta_Case; tea.
+  apply All2_refl. split; reflexivity.
+Defined.
+Hint Resolve beta_eta_Case0 : beta_eta.
+
+Lemma beta_eta_Proj Σ Γ p t0 t1 :
+  beta_eta Σ Γ t0 t1 ->
+  beta_eta Σ Γ (tProj p t0) (tProj p t1).
+Proof.
+  induction 1; beta_eta. destruct r; beta_eta.
+Defined.
+Hint Resolve beta_eta_Proj : beta_eta.
+
+
+Lemma beta_eta_Fix_ty mfix mfix' idx Σ Γ :
+  All2 (fun d0 d1 => beta_eta Σ Γ (dtype d0) (dtype d1)
+                  × dbody d0 = dbody d1
+                  × dname d0 = dname d1
+                  × rarg d0 = rarg d1) mfix mfix' ->
+  beta_eta Σ Γ (tFix mfix idx) (tFix mfix' idx).
+Proof.
+  intro XX.
+  assert (clos_refl_trans (OnOne2 (fun d0 d1 =>
+                  (beta_eta1 Σ Γ (dtype d0) (dtype d1))
+                  × dbody d0 = dbody d1
+                  × dname d0 = dname d1
+                  × rarg d0 = rarg d1)) mfix mfix') as YY; [|clear XX]. {
+    induction XX; [reflexivity|].
+    transitivity (y :: l).
+    - rdestruct r. destruct x, y; cbn in *; subst.
+      induction r.
+      + constructor. now constructor.
+      + reflexivity.
+      + etransitivity; eassumption.
+    - clear XX. induction IHXX.
+      + constructor. now constructor.
+      + reflexivity.
+      + etransitivity; eassumption. }
+  induction YY; beta_eta.
+  assert (((OnOne2 (on_Trel_eq (red1 Σ Γ) dtype
+                      (fun x0 => (dname x0, dbody x0, rarg x0)))) x y)
+          + ((OnOne2 (on_Trel_eq eta1 dtype
+                        (fun x0 => (dname x0, dbody x0, rarg x0)))) x y)) as ZZ. {
+    induction r.
+    - destruct p as [[] ?]; [left|right]; constructor; now split.
+    - destruct IHr; [left|right]; now constructor.
+  }
+  destruct ZZ; beta_eta.
+Qed.
+
+Lemma beta_eta_Fix_bo mfix mfix' idx Σ Γ :
+  All2 (fun d0 d1 => beta_eta Σ (Γ ,,, fix_context mfix) (dbody d0) (dbody d1)
+                  × dtype d0 = dtype d1
+                  × dname d0 = dname d1
+                  × rarg d0 = rarg d1) mfix mfix' ->
+  beta_eta Σ Γ (tFix mfix idx) (tFix mfix' idx).
+Proof.
+  intro XX.
+  assert (clos_refl_trans (OnOne2 (fun d0 d1 =>
+                  beta_eta1 Σ (Γ ,,, fix_context mfix) (dbody d0) (dbody d1)
+                  × dtype d0 = dtype d1
+                  × dname d0 = dname d1
+                  × rarg d0 = rarg d1)) mfix mfix') as YY; [|clear XX]. {
+    set (Γ' := Γ ,,, fix_context mfix) in *; clearbody Γ'.
+    induction XX; [reflexivity|].
+    transitivity (y :: l).
+    - rdestruct r. destruct x, y; cbn in *; subst.
+      induction r.
+      + constructor. now constructor.
+      + reflexivity.
+      + etransitivity; eassumption.
+    - clear XX. induction IHXX.
+      + constructor. now constructor.
+      + reflexivity.
+      + etransitivity; eassumption. }
+  generalize_eq Γ' (fix_context mfix).
+  dependent induction YY; trea.
+  2: { intro e; etransitivity; eauto. apply IHYY2.
+       rewrite e. clear -YY1. induction YY1; [|easy..].
+       apply (f_equal (@List.rev _)). unfold mapi.
+       generalize 0 at 2 4 as k.
+       induction r; intro k; simpl.
+       + rdest. congruence.
+       + now rewrite IHr. }
+  assert (((OnOne2 (on_Trel_eq (red1 Σ (Γ ,,, Γ')) dbody
+                      (fun x0 => (dname x0, dtype x0, rarg x0)))) x y)
+          + ((OnOne2 (on_Trel_eq eta1 dbody
+                        (fun x0 => (dname x0, dtype x0, rarg x0)))) x y)) as ZZ. {
+    induction r.
+    - destruct p as [[] ?]; [left|right]; constructor; now split.
+    - destruct IHr; [left|right]; now constructor.
+  }
+  intro; subst; destruct ZZ; beta_eta.
+Qed.
+
+Lemma beta_eta_Fix mfix mfix' idx Σ Γ :
+  All2 (fun d0 d1 => beta_eta Σ Γ (dtype d0) (dtype d1)
+                  × beta_eta Σ (Γ ,,, fix_context mfix) (dbody d0) (dbody d1)
+                  × dname d0 = dname d1
+                  × rarg d0 = rarg d1) mfix mfix' ->
+  beta_eta Σ Γ (tFix mfix idx) (tFix mfix' idx).
+Proof.
+  intro h.
+  assert (∑ mfixi, All2 (fun d0 d1 =>
+     beta_eta Σ (Γ ,,, fix_context mfix) (dbody d0) (dbody d1)
+     × dtype d0 = dtype d1 × dname d0 = dname d1 × rarg d0 = rarg d1) mfix mfixi
+                 × All2 (fun d0 d1 =>
+     beta_eta Σ Γ (dtype d0) (dtype d1)
+     × dbody d0 = dbody d1 × dname d0 = dname d1 × rarg d0 = rarg d1) mfixi mfix'
+         ) as [mfixi [h1 h2]].
+  { revert h. generalize (Γ ,,, fix_context mfix). intros Δ h.
+    induction h.
+    - exists []. auto.
+    - destruct r as [? [? e]]. inversion e.
+      destruct IHh as [mfixi [? ?]].
+      eexists (mkdef _ _ _ _ _ :: mfixi). split.
+      + constructor ; auto. simpl. split ; eauto.
+      + constructor ; auto. }
+  etransitivity.
+  - eapply beta_eta_Fix_bo. eassumption.
+  - eapply beta_eta_Fix_ty. assumption.
+Qed.
+Hint Resolve beta_eta_Fix_ty beta_eta_Fix_bo beta_eta_Fix : beta_eta.
+
+
+Lemma beta_eta_CoFix_ty mfix mfix' idx Σ Γ :
+  All2 (fun d0 d1 => beta_eta Σ Γ (dtype d0) (dtype d1)
+                  × dbody d0 = dbody d1
+                  × dname d0 = dname d1
+                  × rarg d0 = rarg d1) mfix mfix' ->
+  beta_eta Σ Γ (tCoFix mfix idx) (tCoFix mfix' idx).
+Proof.
+  intro XX.
+  assert (clos_refl_trans (OnOne2 (fun d0 d1 =>
+                  (beta_eta1 Σ Γ (dtype d0) (dtype d1))
+                  × dbody d0 = dbody d1
+                  × dname d0 = dname d1
+                  × rarg d0 = rarg d1)) mfix mfix') as YY; [|clear XX]. {
+    induction XX; [reflexivity|].
+    transitivity (y :: l).
+    - rdestruct r. destruct x, y; cbn in *; subst.
+      induction r.
+      + constructor. now constructor.
+      + reflexivity.
+      + etransitivity; eassumption.
+    - clear XX. induction IHXX.
+      + constructor. now constructor.
+      + reflexivity.
+      + etransitivity; eassumption. }
+  induction YY; beta_eta.
+  assert (((OnOne2 (on_Trel_eq (red1 Σ Γ) dtype
+                      (fun x0 => (dname x0, dbody x0, rarg x0)))) x y)
+          + ((OnOne2 (on_Trel_eq eta1 dtype
+                        (fun x0 => (dname x0, dbody x0, rarg x0)))) x y)) as ZZ. {
+    induction r.
+    - destruct p as [[] ?]; [left|right]; constructor; now split.
+    - destruct IHr; [left|right]; now constructor.
+  }
+  destruct ZZ; beta_eta.
+Qed.
+
+Lemma beta_eta_CoFix_bo mfix mfix' idx Σ Γ :
+  All2 (fun d0 d1 => beta_eta Σ (Γ ,,, fix_context mfix) (dbody d0) (dbody d1)
+                  × dtype d0 = dtype d1
+                  × dname d0 = dname d1
+                  × rarg d0 = rarg d1) mfix mfix' ->
+  beta_eta Σ Γ (tCoFix mfix idx) (tCoFix mfix' idx).
+Proof.
+  intro XX.
+  assert (clos_refl_trans (OnOne2 (fun d0 d1 =>
+                 beta_eta1 Σ (Γ ,,, fix_context mfix) (dbody d0) (dbody d1)
+                  × dtype d0 = dtype d1
+                  × dname d0 = dname d1
+                  × rarg d0 = rarg d1)) mfix mfix') as YY; [|clear XX]. {
+    set (Γ' := Γ ,,, fix_context mfix) in *; clearbody Γ'.
+    induction XX; [reflexivity|].
+    transitivity (y :: l).
+    - rdestruct r. destruct x, y; cbn in *; subst.
+      induction r.
+      + constructor. now constructor.
+      + reflexivity.
+      + etransitivity; eassumption.
+    - clear XX. induction IHXX.
+      + constructor. now constructor.
+      + reflexivity.
+      + etransitivity; eassumption. }
+  generalize_eq Γ' (fix_context mfix).
+  dependent induction YY; trea.
+  2: { intro e; etransitivity; eauto. apply IHYY2.
+       rewrite e. clear -YY1. induction YY1; [|easy..].
+       apply (f_equal (@List.rev _)). unfold mapi.
+       generalize 0 at 2 4 as k.
+       induction r; intro k; simpl.
+       + rdest. congruence.
+       + now rewrite IHr. }
+  assert (((OnOne2 (on_Trel_eq (red1 Σ (Γ ,,, Γ')) dbody
+                      (fun x0 => (dname x0, dtype x0, rarg x0)))) x y)
+          + ((OnOne2 (on_Trel_eq eta1 dbody
+                        (fun x0 => (dname x0, dtype x0, rarg x0)))) x y)) as ZZ. {
+    induction r.
+    - destruct p as [[] ?]; [left|right]; constructor; now split.
+    - destruct IHr; [left|right]; now constructor.
+  }
+  intro; subst; destruct ZZ; beta_eta.
+Qed.
+
+Lemma beta_eta_CoFix mfix mfix' idx Σ Γ :
+  All2 (fun d0 d1 => beta_eta Σ Γ (dtype d0) (dtype d1)
+                  × beta_eta Σ (Γ ,,, fix_context mfix) (dbody d0) (dbody d1)
+                  × dname d0 = dname d1
+                  × rarg d0 = rarg d1) mfix mfix' ->
+  beta_eta Σ Γ (tCoFix mfix idx) (tCoFix mfix' idx).
+Proof.
+  intro h.
+  assert (∑ mfixi, All2 (fun d0 d1 =>
+     beta_eta Σ (Γ ,,, fix_context mfix) (dbody d0) (dbody d1)
+     × dtype d0 = dtype d1 × dname d0 = dname d1 × rarg d0 = rarg d1) mfix mfixi
+                 × All2 (fun d0 d1 =>
+     beta_eta Σ Γ (dtype d0) (dtype d1)
+     × dbody d0 = dbody d1 × dname d0 = dname d1 × rarg d0 = rarg d1) mfixi mfix'
+         ) as [mfixi [h1 h2]].
+  { revert h. generalize (Γ ,,, fix_context mfix). intros Δ h.
+    induction h.
+    - exists []. auto.
+    - destruct r as [? [? e]]. inversion e.
+      destruct IHh as [mfixi [? ?]].
+      eexists (mkdef _ _ _ _ _ :: mfixi). split.
+      + constructor ; auto. simpl. split ; eauto.
+      + constructor ; auto. }
+  etransitivity.
+  - eapply beta_eta_CoFix_bo. eassumption.
+  - eapply beta_eta_CoFix_ty. assumption.
+Qed.
+Hint Resolve beta_eta_CoFix_ty beta_eta_CoFix_bo beta_eta_CoFix : beta_eta.
+
+Lemma beta_eta_mkApps Σ Γ M M' l l' :
+  beta_eta Σ Γ M M' -> All2 (beta_eta Σ Γ) l l' ->
+  beta_eta Σ Γ (mkApps M l) (mkApps M' l').
+Proof.
+  intros X Y.
+  induction Y in M, M', X |- * ; cbn; beta_eta.
+Qed.
+Hint Resolve beta_eta_mkApps : beta_eta.
+
+ 
 (** ** Basic Properties of cumul *)
 
 Instance cumul_refl' {cf:checker_flags} Σ Γ : Reflexive (cumul Σ Γ).
 Proof.
-  intro; econstructor; reflexivity.
+  intro x; repeat exists x; repeat split; reflexivity.
 Qed.
 
 Instance conv_refl' {cf:checker_flags} Σ Γ : Reflexive (conv Σ Γ).
 Proof.
-  intro; econstructor; reflexivity.
+  intro x; repeat exists x; repeat split; reflexivity.
 Qed.
 
-Lemma red_cumul_cumul {cf:checker_flags} {Σ : global_env_ext} {Γ t u v} :
-  red Σ Γ t u -> Σ ;;; Γ |- u <= v -> Σ ;;; Γ |- t <= v.
-Proof.
-  induction 1 in v |- *; auto.
-  intro. apply IHX. econstructor 2; eassumption.
-Qed.
+(* Lemma red_cumul_cumul {cf:checker_flags} {Σ : global_env_ext} {Γ t u v} : *)
+(*   red Σ Γ t u -> Σ ;;; Γ |- u <= v -> Σ ;;; Γ |- t <= v. *)
+(* Proof. *)
+(*   induction 1 in v |- *; auto. *)
+(*   intro. apply IHX. econstructor 2; eassumption. *)
+(* Qed. *)
 
-Lemma red_cumul_cumul_inv {cf:checker_flags} {Σ : global_env_ext} {Γ t u v} :
-  red Σ Γ t v -> Σ ;;; Γ |- u <= v -> Σ ;;; Γ |- u <= t.
-Proof.
-  induction 1 in u |- *; auto.
-  intro. apply IHX. econstructor 3; eassumption.
-Qed.
+(* Lemma red_cumul_cumul_inv {cf:checker_flags} {Σ : global_env_ext} {Γ t u v} : *)
+(*   red Σ Γ t v -> Σ ;;; Γ |- u <= v -> Σ ;;; Γ |- u <= t. *)
+(* Proof. *)
+(*   induction 1 in u |- *; auto. *)
+(*   intro. apply IHX. econstructor 3; eassumption. *)
+(* Qed. *)
 
 Lemma red_cumul {cf:checker_flags} {Σ : global_env_ext} {Γ t u} :
   red Σ Γ t u ->
   Σ ;;; Γ |- t <= u.
 Proof.
-  intro; eapply red_cumul_cumul; tea; reflexivity.
+  intros; repeat eexists; repeat split.
+  2: eapply red_beta_eta; eassumption.
+  all: reflexivity.
 Qed.
 
 Lemma red_cumul_inv {cf:checker_flags} {Σ : global_env_ext} {Γ t u} :
   red Σ Γ t u ->
   Σ ;;; Γ |- u <= t.
 Proof.
-  intro; eapply red_cumul_cumul_inv; tea; reflexivity.
+  intros; repeat eexists; repeat split.
+  4: eapply red_beta_eta; eassumption.
+  all: reflexivity.
 Qed.
 
 
 (** ** Basic Properties of conv *)
 
-Lemma red_conv_conv `{cf : checker_flags} Σ Γ t u v :
-  red (fst Σ) Γ t u -> Σ ;;; Γ |- u = v -> Σ ;;; Γ |- t = v.
-Proof.
-  induction 1 in v |- *; auto.
-  intro. apply IHX. econstructor 2; eassumption.
-Qed.
+(* Lemma red_conv_conv `{cf : checker_flags} Σ Γ t u v : *)
+(*   red (fst Σ) Γ t u -> Σ ;;; Γ |- u = v -> Σ ;;; Γ |- t = v. *)
+(* Proof. *)
+(*   induction 1 in v |- *; auto. *)
+(*   intro. apply IHX. econstructor 2; eassumption. *)
+(* Qed. *)
 
-Lemma red_conv_conv_inv `{cf : checker_flags} Σ Γ t u v :
-  red (fst Σ) Γ t u -> Σ ;;; Γ |- v = u -> Σ ;;; Γ |- v = t.
-Proof.
-  induction 1 in v |- *; auto.
-  intro. apply IHX. econstructor 3; eassumption.
-Qed.
+(* Lemma red_conv_conv_inv `{cf : checker_flags} Σ Γ t u v : *)
+(*   red (fst Σ) Γ t u -> Σ ;;; Γ |- v = u -> Σ ;;; Γ |- v = t. *)
+(* Proof. *)
+(*   induction 1 in v |- *; auto. *)
+(*   intro. apply IHX. econstructor 3; eassumption. *)
+(* Qed. *)
 
 Lemma red_conv {cf:checker_flags} (Σ : global_env_ext) Γ t u :
   red Σ Γ t u -> Σ ;;; Γ |- t = u.
 Proof.
-  intro; now eapply red_conv_conv.
+  intros; repeat eexists; repeat split.
+  2: eapply red_beta_eta; eassumption.
+  all: reflexivity.
 Qed.
 
 Lemma red_conv_inv {cf:checker_flags} (Σ : global_env_ext) Γ t u :
   red Σ Γ t u -> Σ ;;; Γ |- u = t.
 Proof.
-  intro; now eapply red_conv_conv_inv.
+  intros; repeat eexists; repeat split.
+  4: eapply red_beta_eta; eassumption.
+  all: reflexivity.
 Qed.
 
 
