pcuic/theories/PCUICConfluence.v
@@ -955,7 +955,6 @@ Section RedEq.
     ∑ T', red Σ Γ T T' * eq_term_upto_univ Re Rle T' V.
   Proof.
     intros eq r.
-    apply red_alt in r.
     induction r in T, eq |- *.
     - eapply red1_eq_term_upto_univ_r in eq as [v' [r' eq']]; eauto.
     - exists T; split; eauto.
@@ -973,7 +972,6 @@ Section RedEq.
     eq_term_upto_univ Re Rle v v'.
   Proof.
     intros eq r.
-    eapply red_alt in r.
     induction r in u', eq |- *.
     - eapply red1_eq_term_upto_univ_l in eq as [v' [r' eq']]; eauto.
     - exists u'. split; auto.
@@ -1440,12 +1438,8 @@ Section PredRed.
     revert Γ Γ'. eapply (@pred1_ind_all_ctx Σ _
                                             (fun Γ Γ' =>
        All2_local_env (on_decl (fun Γ Γ' M N => pred1 Σ Γ Γ' M N -> red Σ Γ M N)) Γ Γ')%type);
-                   intros; try constructor; pcuic.
+                   intros; try reflexivity; pcuic.
     eapply All2_local_env_impl; eauto.
-    - (* Contexts *)
-      unfold on_decl => Δ Δ' t T U Hlen.
-      destruct t; auto.
-      destruct p; auto. intuition.
 
     - (* Beta *)
       apply red_trans with (tApp (tLambda na t0 b1) a0).
@@ -1578,11 +1572,8 @@ Section PredRed.
        _ _ _ _ _ _ _ _ _ _ _ _ _ _ _ _ _ _ _ _ _ _);
       intros; subst; try solve [econstructor; eauto].
 
-    - eapply (All2_local_env_impl _ _ _ _ X0). clear X0; intros.
-      red in X0 |- *.
-      destruct t as [[t t']|].
-      intuition subst. specialize (a Γ1 Γ'0 Δ0 Δ' eq_refl eq_refl). eauto.
-      eapply b; eauto. intros; subst. eapply X0; eauto.
+    - eapply (All2_local_env_impl X0). clear X0; intros.
+      eapply X0; tea.
     
     - econstructor; eauto. 
       specialize (X0 Γ0 Γ'0 (Δ ,, vass na t0) (Δ' ,, vass na t1) eq_refl).
@@ -2032,8 +2023,7 @@ Section RedConfluence.
     red Σ Γ t u ->
     trans_clos pred1_rel (Γ, t) (Γ, u).
   Proof.
-    move/(equiv _ _ (red_alt _ _ _ _)) => tu.
-    induction tu.
+    induction 1.
     constructor. now eapply red1_pred1 in r.
     constructor. pcuic.
     econstructor 2; eauto.
@@ -2196,13 +2186,12 @@ Section RedConfluence.
     red in p.
     transitivity (Γ ,, vass na t').
     eapply clos_rt_OnOne2_local_env_ctx_incl, clos_rt_OnOne2_local_env_incl. constructor. red.
-    eapply red_alt in p; eauto.
+    eauto.
     clear p H.
     transitivity (Γ ,, vass na' t').
     { constructor 2. repeat constructor; auto. apply reflexivity. }
     induction IHAll2_local_env; try solve[repeat constructor; auto].
     etransitivity; eauto.
-    apply red_alt in a. apply red_alt in b0.
     transitivity (Γ ,, vdef na b t').
     - eapply clos_rt_OnOne2_local_env_ctx_incl, clos_rt_OnOne2_local_env_incl. constructor 2. red.
       right. split; auto.
@@ -2275,7 +2264,6 @@ Section RedConfluence.
   Lemma clos_rt_red1_rel_ctx_rt_ctx_red1_rel : inclusion red_rel_ctx (clos_refl_trans_ctx_t red1_rel).
   Proof.
     move=> [Γ t] [Δ u] [redt redctx].
-    eapply red_alt in redt.
     eapply clos_rt_rt1n_iff in redt.
     induction redt.
     induction redctx; try solve [constructor; eauto].
@@ -2283,23 +2271,21 @@ Section RedConfluence.
     - red in p.
       etransitivity.
       * eapply clos_rt_ctx_t_disjunction_right.
-        eapply red_alt in p. instantiate (1:= (Γ',, vass na' t', x)).
+        instantiate (1:= (Γ',, vass na' t', x)).
         eapply clos_refl_trans_ctx_t_prod_l. intros. split; eauto.
         transitivity (Γ ,, vass na' t).
         constructor 2. repeat constructor; apply reflexivity.
         apply red_ctx_clos_rt_red1_ctx. constructor; auto.
-        red. apply red_alt; auto.
       * clear p. eapply clos_rt_ctx_t_disjunction_right.
         constructor 2; simpl; apply reflexivity.
     - red in p.
       destruct p.
-      eapply red_alt in r. eapply red_alt in r0.
       etransitivity.
       * eapply clos_rt_ctx_t_disjunction_right.
         instantiate (1:= (Γ',, vdef na b' t', x)).
         eapply clos_refl_trans_ctx_t_prod_l. intros. split; eauto.
         apply red_ctx_clos_rt_red1_ctx. constructor; auto.
-        red. split; apply red_alt; auto.
+        red. split; auto.
       * clear r r0.
         eapply clos_rt_ctx_t_disjunction_right.
         eapply clos_refl_trans_ctx_t_prod_l. intros. split; eauto.
@@ -2350,7 +2336,7 @@ Section RedConfluence.
     transitivity (c, t0).
     eapply clos_rt_disjunction_left.
     eapply clos_refl_trans_prod_r. intros. split; eauto.
-    now eapply red_alt in r.
+    assumption.
     eapply clos_rt_disjunction_right.
     eapply (clos_refl_trans_prod_l (fun x y => red1_ctx x y + eq_context_upto_names x y))%type.
     intros. red. destruct X; intuition auto.
@@ -2382,8 +2368,7 @@ Section RedConfluence.
     red_ctx Δ Γ ->
     red Σ Δ t u.
   Proof.
-    move=> H Hctx. apply red_alt in H.
-    induction H.
+    move=> H Hctx. induction H.
     revert Δ Hctx.
     induction r using red1_ind_all; intros Δ Hctx; try solve [eapply red_step; repeat (constructor; eauto)].
     - red in Hctx.
@@ -2395,10 +2380,10 @@ Section RedConfluence.
       rewrite firstn_length_le //.
       destruct (nth_error Δ) eqn:Heq => //.
       eapply nth_error_Some_length in Heq. lia.
-    - eapply red_step; repeat (econstructor; eauto).
-    - eapply red_step; repeat (econstructor; eauto).
-    - eapply red_step; repeat (econstructor; eauto).
-    - eapply red_step; repeat (econstructor; eauto).
+    - eapply red_step; now repeat (econstructor; eauto).
+    - eapply red_step; now repeat (econstructor; eauto).
+    - eapply red_step; now repeat (econstructor; eauto).
+    - eapply red_step; now repeat (econstructor; eauto).
     - eapply red_abs_alt. eauto. eauto.
     - eapply red_abs_alt. eauto. apply (IHr (Δ ,, vass na N)).
       constructor; auto. red. auto.
@@ -2508,7 +2493,7 @@ Section RedConfluence.
     apply red1_rel_alpha_red1_rel_inv.
     transitivity (Γ, u).
     eapply clos_refl_trans_ctx_t_prod_r. intros. red. left. split; eauto.
-    apply red_alt. now apply pred1_red in r.
+    now apply pred1_red in r.
     eapply clos_refl_trans_ctx_t_prod_l. intros. red. right. split; eauto.
     now apply red_ctx_clos_rt_red1_ctx, pred1_ctx_red_ctx.
     constructor 2.
@@ -2557,7 +2542,6 @@ Section RedConfluence.
         apply red1_ctx_pred1_ctx in r.
         apply pred1_ctx_red_ctx in r.
         etransitivity; eauto.
-        apply red_alt in c. apply red_alt.
         eapply red_red_ctx; eauto.
         apply red1_ctx_pred1_ctx in r.
         now apply pred1_ctx_red_ctx in r.
@@ -2629,7 +2613,7 @@ Section RedConfluence.
     red Σ Γ t u ->
     red Σ Γ' t u.
   Proof.
-    intros HΓ H. apply red_alt in H. apply red_alt.
+    intros HΓ H.
     move: H. apply clos_rt_monotone => x y.
     now apply red1_eq_context_upto_names.
   Qed.
@@ -2684,7 +2668,6 @@ Section RedConfluence.
         apply red1_ctx_pred1_ctx in r.
         apply pred1_ctx_red_ctx in r.
         etransitivity; eauto.
-        apply red_alt in c. apply red_alt.
         eapply red_red_ctx; eauto.
         apply red1_ctx_pred1_ctx in r.
         now apply pred1_ctx_red_ctx in r.
@@ -2714,10 +2697,9 @@ Section RedConfluence.
     red Σ (Γ ,,, Δ') t u.
   Proof.
     intros redt assΔ redΔ.
-    eapply red_alt in redt.
     induction redt.
     - eapply red1_red1_ctx_inv; eauto.
-    - constructor.
+    - reflexivity.
     - now transitivity y.
   Qed.
     
@@ -2794,8 +2776,7 @@ Section ConfluenceFacts.
     ∑ args' : list term,
     (c = mkApps (tConstruct ind pars k) args') * (All2 (red Σ Γ) args args').
   Proof.
-    move => Hred. apply red_alt in Hred.
-    eapply red_pred in Hred.
+    move => Hred. eapply red_pred in Hred.
     generalize_eq x (mkApps (tConstruct ind pars k) args).
     induction Hred in ind, pars, k, args |- * ; simplify *.
     - eapply pred1_mkApps_tConstruct in r as [r' [eq redargs]].
@@ -2814,8 +2795,7 @@ Section ConfluenceFacts.
     ∑ args' : list term,
     (c = mkApps (tInd ind u) args') * (All2 (red Σ Γ) args args').
   Proof.
-    move => Hred. apply red_alt in Hred.
-    eapply red_pred in Hred; tas.
+    move => Hred. eapply red_pred in Hred; tas.
     generalize_eq x (mkApps (tInd ind u) args).
     induction Hred in ind, u, args |- * ; simplify *.
     - eapply pred1_mkApps_tInd in r as [r' [eq redargs]].
@@ -2834,8 +2814,7 @@ Section ConfluenceFacts.
     ∑ args' : list term,
     (c = mkApps (tConst cst u) args') * (All2 (red Σ Γ) args args').
   Proof.
-    move => Hdecl Hbody Hred. apply red_alt in Hred.
-    eapply red_pred in Hred; tas.
+    move => Hdecl Hbody Hred. eapply red_pred in Hred; tas.
     generalize_eq x (mkApps (tConst cst u) args).
     induction Hred in cst, u, args, Hdecl |- *; simplify *.
     - eapply pred1_mkApps_tConst_axiom in r as [r' [eq redargs]]; eauto.
@@ -2861,9 +2840,8 @@ Section ConfluenceFacts.
     red Σ Γ t u -> red Σ Γ t v ->
     ∑ v', red Σ Γ u v' * red Σ Γ v v'.
   Proof.
-    move=> H H'. apply red_alt in H. apply red_alt in H'.
+    move=> H H'.
     destruct (red1_confluent wfΣ _ _ _ _ H H') as [nf [redl redr]].
-    apply red_alt in redl; apply red_alt in redr.
     exists nf; intuition auto.
   Qed.
 
